Fix compile problems

theories/Handlers/Deterministic.v
@@ -1,5 +1,5 @@
 (* SLOT, a formally verified model checker
-   Copyright (C) 2019-2021  k32
+   Copyright (C) 2019-2023  k32
 
    This program is free software: you can redistribute it and/or modify
    it under the terms of the GNU General Public License as published by
@@ -49,25 +49,25 @@ Module Var.
   Section defs.
     Context {T : Type}.
 
-    Inductive var_req_t :=
+    Inductive req_t :=
     | read
-    | write : T -> var_req_t.
+    | write : T -> req_t.
 
-    Definition var_ret_t req :=
+    Definition ret_t req :=
       match req with
       | read => T
       | write _ => True
       end.
 
-    Definition var_step (_ : PID) s req : T * var_ret_t req :=
+    Definition step (_ : PID) s req : T * ret_t req :=
       match req with
       | read => (s, s)
       | write new => (new, I)
       end.
 
-    Global Instance varDetHandler : DeterministicHandler var_req_t var_ret_t :=
+    Global Instance varDetHandler : DeterministicHandler req_t ret_t :=
       { det_h_state := T;
-        det_h_state_transition := var_step;
+        det_h_state_transition := step;
       }.
   End defs.
 
@@ -95,11 +95,13 @@ Module Log.
 
     Definition State : Type := list Event.
 
-    Definition hist_req_t := PID -> Event.
+    Definition req_t := PID -> Event.
 
-    Definition step (pid : PID) (s : State) (req : hist_req_t) := (req pid :: s, I).
+    Definition ret_t := I.
 
-    Global Instance historyDetHandler : DeterministicHandler hist_req_t (fun _ => True) :=
+    Definition step (pid : PID) (s : State) (req : req_t) := (req pid :: s, ret_t).
+
+    Global Instance historyDetHandler : DeterministicHandler req_t (fun _ => True) :=
       { det_h_state := list Event;
         det_h_state_transition := step;
       }.
