theories/Handlers.v
@@ -1,5 +1,5 @@
 (* SLOT, a formally verified model checker
-   Copyright (C) 2019-2021  k32
+   Copyright (C) 2019-2023  k32
 
    This program is free software: you can redistribute it and/or modify
    it under the terms of the GNU General Public License as published by
@@ -124,4 +124,4 @@ Ltac decompose_state :=
            destruct H as [l r]; simpl in l,r
          end.
 
-Hint Transparent compose_state : slot.
+#[export] Hint Transparent compose_state : slot.
