theories/Handlers/Mutex.v
@@ -1,5 +1,5 @@
 (* SLOT, a formally verified model checker
-   Copyright (C) 2019-2021  k32
+   Copyright (C) 2019-2023  k32
 
    This program is free software: you can redistribute it and/or modify
    it under the terms of the GNU General Public License as published by
@@ -82,7 +82,7 @@ Ltac mutex_contradiction :=
       inversion H1; inversion H2; subst; discriminate
   end.
 
-Hint Extern 4 => mutex_contradiction : handlers.
+#[export] Hint Extern 4 => mutex_contradiction : handlers.
 
 Ltac clear_mutex :=
   repeat match goal with
